_Harkeerat Singh Sawhney & Mak Fazlic_

## Problem 1. (Error propagation)

Assuming that $\big |\frac{\triangle x}{x}|, \big |\frac{\triangle y}{y}| <<1$﻿.

### **a) Prove that** **$\frac{((x + \triangle x) + (y + \triangle y)) - (x + y)}{x+y} = \frac{x}{x+y}\frac{\triangle x}{x} + \frac{y}{x+y}\frac{\triangle y}{y} $**﻿

Hence in order to first solve this lets simplify $\frac{((x + \triangle x) + (y + \triangle y)) - (x + y)}{x+y}$﻿ first.

$\frac{((x + \triangle x) + (y + \triangle y)) - (x + y)}{x+y} = \frac{((x + y) + (\triangle x + \triangle y)) - (x + y)}{x+y} \newline = \frac{\triangle x + \triangle y}{x+y} = \bold{\frac{\triangle x}{x+y} +\frac{\triangle y}{x+y}} \rightarrow \underline{\bold{I}}$

Now, simplifying $\frac{x}{x+y}\frac{\triangle x}{x} + \frac{y}{x+y}\frac{\triangle y}{y} $﻿,

$\frac{x}{x+y}\frac{\triangle x}{x} + \frac{y}{x+y}\frac{\triangle y}{y} = \bold{\frac{\triangle x}{x+y} + \frac{\triangle y}{x+y}} \rightarrow \bold{\underline{II}} $

==Therefore, it has proved the== ==**LHS**== ==and== ==**RHS**== ==are equal, or in order words== ==$\bold{\underline{I}} = \bold{\underline{II}} $==﻿ ==for== ==$x \neq -y, y \neq -x$==﻿

### b) Prove that $\frac{((x + \triangle x) - (y + \triangle y)) - (x + y)}{x+y} = \frac{x}{x+y}\frac{\triangle x}{x} - \frac{y}{x+y}\frac{\triangle y}{y} $﻿

Hence in order to first solve this lets simplify $\frac{((x + \triangle x) + (y + \triangle y)) - (x + y)}{x+y}$﻿ first.

$\frac{((x + \triangle x) - (y + \triangle y)) - (x + y)}{x+y} = \frac{((x - y) + (\triangle x - \triangle y)) - (x - y)}{x+y} \newline = \frac{\triangle x - \triangle y}{x-y} = \bold{\frac{\triangle x}{x-y} -\frac{\triangle y}{x-y}} \rightarrow \underline{\bold{I}}$

Now, simplifying $\frac{x}{x+y}\frac{\triangle x}{x} + \frac{y}{x+y}\frac{\triangle y}{y} $﻿,

$\frac{x}{x-y}\frac{\triangle x}{x} - \frac{y}{x-y}\frac{\triangle y}{y} = \bold{\frac{\triangle x}{x-y} - \frac{\triangle y}{x-y}} \rightarrow \bold{\underline{II}} $

==Therefore, it has proved the== ==**LHS**== ==and== ==**RHS**== ==are equal, or in order words== ==$\bold{\underline{I}} = \bold{\underline{II}} $==﻿ ==for== ==$x \neq y, y \neq x$==